src/reaches.lean
@@ -1,0 +1,360 @@
+import data.pfun
+import logic.relation
+import logic.function.iterate
+
+namespace pfun
+
+/-- Restrict with the intersection of a set -/
+def res_inter {α β : Type*} (f : α →. β) (p : set α) : α →. β :=
+f.restrict (set.inter_subset_right p f.dom)
+
+@[simp] lemma mem_res_inter {α β : Type*} {f : α →. β} {p : set α} {x y} :
+  y ∈ f.res_inter p x ↔ x ∈ p ∧ y ∈ f x :=
+by { simp [res_inter], tauto, }
+
+end pfun
+
+open relation
+open nat (iterate)
+open function (update iterate_succ iterate_succ_apply iterate_succ'
+  iterate_succ_apply' iterate_zero_apply)
+
+namespace part_eval
+
+/-- Run a state transition function `σ → option σ` "to completion". The return value is the last
+state returned before a `none` result. If the state transition function always returns `some` or any step of the
+transition function diverges, then the computation diverges, returning `part.none`. -/
+def eval {σ} (f : σ →. option σ) : σ → part σ :=
+pfun.fix (λ s, (f s).map (λ x, x.elim (sum.inl s) sum.inr))
+
+/-- The reflexive transitive closure of a state transition function. `reaches f a b` means
+there is a finite sequence of steps `f a = some a₁`, `f a₁ = some a₂`, ... such that `aₙ = b`.
+This relation permits zero steps of the state transition function. -/
+def reaches {σ} (f : σ →. option σ) : σ → σ → Prop :=
+refl_trans_gen (λ a b, some b ∈ f a)
+
+@[refl] lemma reaches.refl {σ} (f : σ →. option σ) (x : σ) :
+  reaches f x x := refl_trans_gen.refl
+
+@[trans] lemma reaches.trans {σ} {f : σ →. option σ} {x y z : σ} :
+  reaches f x y → reaches f y z → reaches f x z := refl_trans_gen.trans
+
+lemma reaches_fwd {σ} {f : σ →. option σ} {x y : σ} :
+  some y ∈ f x → reaches f x y := @refl_trans_gen.single _ _ x y
+
+theorem reaches_mono {σ} {f : σ →. option σ} (S : set σ) (hS : S ⊆ f.dom) {x y} (hf : reaches (f.restrict hS) x y) :
+  reaches f x y :=
+by { apply refl_trans_gen.mono _ hf, simp, }
+
+theorem invariant_of_reaches {σ} {f : σ →. option σ} (S : set σ) (hS : ∀ ⦃x y⦄, x ∈ S → some y ∈ f x → y ∈ S)
+  {x y} (hx : x ∈ S) (hf : reaches f x y) : y ∈ S :=
+by { induction hf with x' y' hfx' hfy' ih, { exact hx, }, exact hS ih hfy', }
+
+theorem reaches_of_invariant {σ} {f : σ →. option σ} (S : set σ) (hS : ∀ ⦃x y⦄, x ∈ S → some y ∈ f x → y ∈ S)
+  {x y} (hx : x ∈ S) (hf : reaches f x y) : reaches (f.res_inter S) x y :=
+begin
+  induction hf using relation.refl_trans_gen.head_induction_on with x' y' hx' hy' ih, { refl, },
+  apply reaches.trans (reaches_fwd _) (ih _),
+  { simp only [pfun.mem_res_inter], exact ⟨hx, hx'⟩, }, { exact hS hx hx', }
+end
+
+/-- The transitive closure of a state transition function. `reaches₁ f a b` means there is a
+nonempty finite sequence of steps `f a = some a₁`, `f a₁ = some a₂`, ... such that `aₙ = b`.
+This relation does not permit zero steps of the state transition function. -/
+def reaches₁ {σ} (f : σ →. option σ) : σ → σ → Prop :=
+trans_gen (λ a b, some b ∈ f a)
+
+theorem reaches_iff_eq_or_reaches₁ {σ} {f : σ →. option σ} {a b} :
+  reaches f a b ↔ b = a ∨ reaches₁ f a b := refl_trans_gen_iff_eq_or_trans_gen
+
+theorem reaches₁_head'_iff {σ} {f : σ →. option σ} {a b} :
+  reaches₁ f a b ↔ ∃ c : σ, some c ∈ f a ∧ reaches f c b := trans_gen.head'_iff
+
+theorem reaches₁_eq {σ} {f : σ →. option σ} {a b c}
+  (h : f a = f b) : reaches₁ f a c ↔ reaches₁ f b c :=
+trans_gen.head'_iff.trans (trans_gen.head'_iff.trans $ by rw h).symm
+
+theorem reaches_total {σ} {f : σ →. option σ}
+  {a b c} (hab : reaches f a b) (hac : reaches f a c) :
+  reaches f b c ∨ reaches f c b :=
+refl_trans_gen.total_of_right_unique (λ x y z hx hy, option.some_injective _ (part.mem_unique hx hy)) hab hac
+
+theorem reaches₁_fwd {σ} {f : σ →. option σ}
+  {a b c} (h₁ : reaches₁ f a c) (h₂ : some b ∈ f a) : reaches f b c :=
+begin
+  rw reaches₁_head'_iff at h₁, rcases h₁ with ⟨b', ⟨h₂', H⟩⟩,
+  cases part.mem_unique h₂ h₂', exact H,
+end
+
+theorem reaches₁_single {σ} {f : σ →. option σ}
+  {a b} : some b ∈ f a → reaches₁ f a b :=
+@trans_gen.single σ _ a b
+
+/-- A variation on `reaches`. `reaches₀ f a b` holds if whenever `reaches₁ f b c` then
+`reaches₁ f a c`. This is a weaker property than `reaches` and is useful for replacing states with
+equivalent states without taking a step. -/
+def reaches₀ {σ} (f : σ →. option σ) (a b : σ) : Prop :=
+∀ c, reaches₁ f b c → reaches₁ f a c
+
+theorem reaches₀.trans {σ} {f : σ →. option σ} {a b c : σ}
+  (h₁ : reaches₀ f a b) (h₂ : reaches₀ f b c) : reaches₀ f a c
+| d h₃ := h₁ _ (h₂ _ h₃)
+
+@[refl] theorem reaches₀.refl {σ} {f : σ →. option σ} (a : σ) : reaches₀ f a a
+| b h := h
+
+theorem reaches₀.single {σ} {f : σ →. option σ} {a b : σ}
+  (h : some b ∈ f a) : reaches₀ f a b
+| c h₂ := h₂.head h
+
+theorem reaches₀.head {σ} {f : σ →. option σ} {a b c : σ}
+  (h : some b ∈ f a) (h₂ : reaches₀ f b c) : reaches₀ f a c :=
+(reaches₀.single h).trans h₂
+
+theorem reaches₀.tail {σ} {f : σ →. option σ} {a b c : σ}
+  (h₁ : reaches₀ f a b) (h : some c ∈ f b) : reaches₀ f a c :=
+h₁.trans (reaches₀.single h)
+
+theorem reaches₀_eq {σ} {f : σ →. option σ} {a b}
+  (e : f a = f b) : reaches₀ f a b
+| d h := (reaches₁_eq e).2 h
+
+theorem reaches₁.to₀ {σ} {f : σ →. option σ} {a b : σ}
+  (h : reaches₁ f a b) : reaches₀ f a b
+| c h₂ := h.trans h₂
+
+theorem reaches.to₀ {σ} {f : σ →. option σ} {a b : σ}
+  (h : reaches f a b) : reaches₀ f a b
+| c h₂ := h₂.trans_right h
+
+theorem reaches₀.tail' {σ} {f : σ →. option σ} {a b c : σ}
+  (h : reaches₀ f a b) (h₂ : some c ∈ f b) : reaches₁ f a c :=
+h _ (trans_gen.single h₂)
+
+/-- (co-)Induction principle for `eval`. If a property `C` holds of any point `a` evaluating to `b`
+which is either terminal (meaning `a = b`) or where the next point also satisfies `C`, then it
+holds of any point where `eval f a` evaluates to `b`. This formalizes the notion that if
+`eval f a` evaluates to `b` then it reaches terminal state `b` in finitely many steps. -/
+@[elab_as_eliminator] def eval_induction {σ}
+  {f : σ →. option σ} {b : σ} {C : σ → Sort*} {a : σ} (h : b ∈ eval f a)
+  (H : ∀ a, b ∈ eval f a →
+    (∀ a', f a = part.some (some a') → C a') → C a) : C a :=
+pfun.fix_induction h (λ _ b ih, H _ b (λ _ ha, ih _ (by simp [ha])))
+
+theorem mem_eval {σ} {f : σ →. option σ} {a b} :
+  b ∈ eval f a ↔ reaches f a b ∧ f b = part.some none :=
+begin
+  split,
+  { intro h, 
+    apply eval_induction h, clear h a, intros a hb ih,
+    have : (f a).dom := by simpa using pfun.dom_of_mem_fix hb, 
+    rw part.dom_iff_mem at this,
+    rcases this with ⟨a'|a', ha'⟩, rw ← part.eq_some_iff at ha',
+    { rw [eval] at hb, cases (part.mem_unique hb (pfun.fix_stop a _) : b = a),
+      { exact ⟨by refl, ha'⟩, }, { simp [ha'], } },
+    specialize ih a' (by rwa part.eq_some_iff),
+    exact ⟨(reaches_fwd ha').trans ih.1, ih.2⟩, },
+  { rintro ⟨h₁, h₂⟩,
+    induction h₁ using relation.refl_trans_gen.head_induction_on with a' b' ha' hb ih,
+    { apply pfun.fix_stop, simp [h₂], },
+    rw [eval, pfun.fix_fwd _ b'], { exact ih, },
+    rw ← part.eq_some_iff at ha', simp [ha'], }
+end
+
+theorem eval_maximal₁ {σ} {f : σ →. option σ} {a b : σ}
+  (h : b ∈ eval f a) (c) : ¬ reaches₁ f b c | bc :=
+let ⟨ab, b0⟩ := mem_eval.1 h, ⟨b', h', _⟩ := trans_gen.head'_iff.1 bc in
+by { rw b0 at h', simpa using h', }
+
+theorem eval_maximal {σ} {f : σ →. option σ} {a b}
+  (h : b ∈ eval f a) {c} : reaches f b c ↔ c = b :=
+let ⟨ab, b0⟩ := mem_eval.1 h in
+refl_trans_gen_iff_eq $ λ b' h',
+by { rw b0 at h', simpa using h', }
+
+theorem reaches_eval {σ} {f : σ →. option σ} {a b}
+  (ab : reaches f a b) : eval f a = eval f b :=
+part.ext $ λ c,
+ ⟨λ h, let ⟨ac, c0⟩ := mem_eval.1 h in
+    mem_eval.2 ⟨(or_iff_left_of_imp $ by exact
+      λ cb, (eval_maximal h).1 cb ▸ refl_trans_gen.refl).1
+      (reaches_total ab ac), c0⟩,
+  λ h, let ⟨bc, c0⟩ := mem_eval.1 h in mem_eval.2 ⟨ab.trans bc, c0⟩,⟩
+
+/-- Given a relation `tr : σ₁ → σ₂ → Prop` between state spaces, and state transition functions
+`f₁ : σ₁ → option σ₁` and `f₂ : σ₂ → option σ₂`, `respects f₁ f₂ tr` means that if `tr a₁ a₂` holds
+initially and `f₁` takes a step to `a₂` then `f₂` will take one or more steps before reaching a
+state `b₂` satisfying `tr a₂ b₂`, and if `f₁ a₁` terminates then `f₂ a₂` also terminates.
+Such a relation `tr` is also known as a refinement. -/
+-- def respects {σ₁ σ₂}
+--   (f₁ : σ₁ →. option σ₁) (f₂ : σ₂ →. option σ₂) (tr : σ₁ → σ₂ → Prop) :=
+-- ∀ ⦃a₁ a₂⦄, tr a₁ a₂ → (match f₁ a₁ with
+--   | part.none := f₂ a₂ = part.none 
+--   | part.some (some b₁) := ∃ b₂, tr b₁ b₂ ∧ reaches₁ f₂ a₂ b₂
+--   | part.some none := f₂ a₂ = none
+--   end : Prop)
+
+structure respects {σ₁ σ₂} (f₁ : σ₁ →. option σ₁) (f₂ : σ₂ →. option σ₂) (tr : σ₁ → σ₂ → Prop) : Prop :=
+(dom_of_dom : ∀ ⦃a₁ a₂⦄, tr a₁ a₂ → (f₂ a₂).dom → (f₁ a₁).dom)
+(some_of_some : ∀ ⦃a₁ a₂ b₁⦄, tr a₁ a₂ → some b₁ ∈ (f₁ a₁) → ∃ b₂, tr b₁ b₂ ∧ reaches₁ f₂ a₂ b₂)
+(none_of_none : ∀ ⦃a₁ a₂⦄, tr a₁ a₂ → none ∈ (f₁ a₁) → none ∈ (f₂ a₂))
+
+variables {σ₁ σ₂ : Type*} {f₁ : σ₁ →. option σ₁} {f₂ : σ₂ →. option σ₂} {tr : σ₁ → σ₂ → Prop}
+
+lemma respects.exists_some {a₁ a₂ b₁} (H : respects f₁ f₂ tr) (aa : tr a₁ a₂) (hb₁ : some b₁ ∈ f₁ a₁) :
+  ∃ b₂, some b₂ ∈ f₂ a₂ :=
+by { obtain ⟨b₂, ⟨_, hb₂⟩⟩ := H.some_of_some aa hb₁, rw reaches₁_head'_iff at hb₂, tauto, }
+
+lemma respects.dom_iff_domm {a₁ a₂} (H : respects f₁ f₂ tr) (aa : tr a₁ a₂) :
+  (f₁ a₁).dom ↔ (f₂ a₂).dom :=
+begin
+  refine ⟨λ h, _, H.dom_of_dom aa⟩,
+  rw [part.dom_iff_mem] at h ⊢, cases h with b₁ hb,
+  cases b₁,
+  { use none, exact H.none_of_none aa hb, },
+  { obtain ⟨b₂, hb₂⟩ := H.exists_some aa hb, exact ⟨_, hb₂⟩, }
+end
+
+lemma respects.none_iff_none {a₁ a₂} (H : respects f₁ f₂ tr) (aa : tr a₁ a₂) :
+  none ∈ f₁ a₁ ↔ none ∈ f₂ a₂ :=
+begin
+  refine ⟨H.none_of_none aa, λ h, _⟩,
+  obtain ⟨x, hx⟩ : ∃ x, x ∈ f₁ a₁, { rw [← part.dom_iff_mem, H.dom_iff_domm aa, part.dom_iff_mem], exact ⟨_, h⟩, },
+  cases x, { exact hx, },
+  obtain ⟨_, hb⟩ := H.exists_some aa hx, cases part.mem_unique h hb,
+end
+
+lemma respects.some_iff_some {a₁ a₂} (H : respects f₁ f₂ tr) (aa : tr a₁ a₂) :
+  (∃ b₁, some b₁ ∈ f₁ a₁) ↔ (∃ b₂, some b₂ ∈ f₂ a₂) :=
+begin
+  refine ⟨λ ⟨b₁, hb₁⟩, H.exists_some aa hb₁, _⟩,
+  rintro ⟨b₂, hb₂⟩,
+  obtain ⟨x, hx⟩ : ∃ x, x ∈ f₁ a₁, { rw [← part.dom_iff_mem, H.dom_iff_domm aa, part.dom_iff_mem], exact ⟨_, hb₂⟩, },
+  cases x, { rw H.none_iff_none aa at hx, cases part.mem_unique hb₂ hx, },
+  exact ⟨_, hx⟩,
+end 
+
+theorem tr_reaches₁
+  (H : respects f₁ f₂ tr) {a₁ a₂} (aa : tr a₁ a₂) {b₁} (ab : reaches₁ f₁ a₁ b₁) :
+  ∃ b₂, tr b₁ b₂ ∧ reaches₁ f₂ a₂ b₂ :=
+begin
+  induction ab with c₁ ac c₁ d₁ ac cd IH,
+  { exact H.some_of_some aa ac, },
+  { rcases IH with ⟨c₂, cc, ac₂⟩,
+    obtain ⟨b₂, ⟨h₁, h₂⟩⟩ := H.some_of_some cc cd,
+    exact ⟨b₂, ⟨h₁, ac₂.trans h₂⟩⟩, }
+end
+
+theorem tr_reaches {σ₁ σ₂ f₁ f₂} {tr : σ₁ → σ₂ → Prop}
+  (H : respects f₁ f₂ tr) {a₁ a₂} (aa : tr a₁ a₂) {b₁} (ab : reaches f₁ a₁ b₁) :
+  ∃ b₂, tr b₁ b₂ ∧ reaches f₂ a₂ b₂ :=
+begin
+  rcases refl_trans_gen_iff_eq_or_trans_gen.1 ab with rfl | ab,
+  { exact ⟨_, aa, refl_trans_gen.refl⟩ },
+  { exact let ⟨b₂, bb, h⟩ := tr_reaches₁ H aa ab in
+    ⟨b₂, bb, h.to_refl⟩ }
+end
+
+theorem tr_reaches_rev {σ₁ σ₂ f₁ f₂} {tr : σ₁ → σ₂ → Prop}
+  (H : respects f₁ f₂ tr) {a₁ a₂} (aa : tr a₁ a₂) {b₂} (ab : reaches f₂ a₂ b₂) :
+  ∃ c₁ c₂, reaches f₂ b₂ c₂ ∧ tr c₁ c₂ ∧ reaches f₁ a₁ c₁ :=
+begin
+  induction ab with a₂' a₂'' ha₂ ha₂' ih,
+  { refine ⟨a₁, a₂, _, aa, _⟩; refl, },
+  rcases ih with ⟨c₁, c₂, c₂h, trh, c₁h⟩,
+  by_cases H : c₂ = a₂',
+  { subst H, clear c₂h,
+    obtain ⟨c₁', hc₁'⟩ := (H.some_iff_some trh).mpr ⟨_, ha₂'⟩,
+    obtain ⟨c₂', hc₂, hc₂'⟩ := H.some_of_some trh hc₁', 
+    exact ⟨c₁', c₂', reaches₁_fwd hc₂' ha₂', hc₂, c₁h.trans (reaches_fwd hc₁')⟩, },
+  refine ⟨c₁, c₂, _, trh, c₁h⟩,
+  simp_rw [reaches_iff_eq_or_reaches₁, H, false_or] at c₂h,
+  apply reaches₁_fwd c₂h ha₂',
+end
+
+theorem tr_eval {σ₁ σ₂ f₁ f₂} {tr : σ₁ → σ₂ → Prop}
+  (H : respects f₁ f₂ tr) {a₁ b₁ a₂} (aa : tr a₁ a₂)
+  (ab : b₁ ∈ eval f₁ a₁) : ∃ b₂, tr b₁ b₂ ∧ b₂ ∈ eval f₂ a₂ :=
+begin
+  cases mem_eval.1 ab with ab b0,
+  rcases tr_reaches H aa ab with ⟨b₂, bb, ab⟩,
+  refine ⟨_, bb, mem_eval.2 ⟨ab, _⟩⟩,
+  rw part.eq_some_iff at ⊢ b0, rwa ← H.none_iff_none bb,
+end
+
+theorem tr_eval_rev {σ₁ σ₂ f₁ f₂} {tr : σ₁ → σ₂ → Prop}
+  (H : respects f₁ f₂ tr) {a₁ b₂ a₂} (aa : tr a₁ a₂)
+  (ab : b₂ ∈ eval f₂ a₂) : ∃ b₁, tr b₁ b₂ ∧ b₁ ∈ eval f₁ a₁ :=
+begin
+  cases mem_eval.1 ab with ab b0,
+  rcases tr_reaches_rev H aa ab with ⟨c₁, c₂, bc, cc, ac⟩,
+  cases (refl_trans_gen_iff_eq _).1 bc,
+  swap, { intros _ h, rw b0 at h, simpa using h, },
+  refine ⟨_, cc, mem_eval.2 ⟨ac, _⟩⟩,
+  rw part.eq_some_iff at b0 ⊢, rwa H.none_iff_none cc,
+end
+
+theorem tr_eval_dom {σ₁ σ₂ f₁ f₂} {tr : σ₁ → σ₂ → Prop}
+  (H : respects f₁ f₂ tr) {a₁ a₂} (aa : tr a₁ a₂) :
+  (eval f₂ a₂).dom ↔ (eval f₁ a₁).dom :=
+⟨λ h, let ⟨b₂, tr, h, _⟩ := tr_eval_rev H aa ⟨h, rfl⟩ in h,
+ λ h, let ⟨b₂, tr, h, _⟩ := tr_eval H aa ⟨h, rfl⟩ in h⟩
+
+/-- A simpler version of `respects` when the state transition relation `tr` is a function. -/
+structure frespects {σ₁ σ₂} (f₁ : σ₁ →. option σ₁) (f₂ : σ₂ →. option σ₂) (tr : σ₁ → σ₂) : Prop :=
+(dom_of_dom : ∀ ⦃a : σ₁⦄, (f₂ (tr a)).dom → (f₁ a).dom)
+(some_of_some : ∀ ⦃a b : σ₁⦄, some b ∈ f₁ a → reaches₁ f₂ (tr a) (tr b))
+(none_of_none : ∀ ⦃a⦄, none ∈ f₁ a → none ∈ f₂ (tr a))
+
+variable {ftr : σ₁ → σ₂}
+theorem fun_respects : respects f₁ f₂ (λ a b, ftr a = b) ↔ frespects f₁ f₂ ftr :=
+begin
+  split,
+  { intro H,
+    refine ⟨λ a, H.dom_of_dom rfl, λ a b hab, _, λ a ha, H.none_of_none rfl ha⟩, 
+    simpa using H.some_of_some rfl hab, },
+  { intro H,
+    refine ⟨_, _, _⟩, { rintro a₁ a₂ rfl h, exact H.dom_of_dom h, },
+    { rintro a₁ a₂ b₁ rfl h, exact ⟨_, rfl, H.some_of_some h⟩, },
+    rintro a₁ a₂ rfl h, exact H.none_of_none h, }
+end
+
+theorem frespects.eval_eq (H : frespects f₁ f₂ ftr)
+  (a₁ : σ₁) : eval f₂ (ftr a₁) = (eval f₁ a₁).map ftr :=
+begin
+  rw ← fun_respects at H,
+  apply part.ext', { exact tr_eval_dom H rfl, },
+  intros h₂ h₁, simp at h₁,
+  have := tr_eval H rfl (part.get_mem h₁),
+  simp at this ⊢, rwa part.get_eq_iff_mem,
+end
+
+def with_time {σ} (f : σ →. option σ) : ℕ × σ →. option (ℕ × σ) :=
+λ tx, (f tx.2).map $ λ x, x.map (λ x', (tx.1+1, x')) 
+
+theorem with_time_frespects {σ} (f : σ →. option σ) :
+  frespects (with_time f) f prod.snd :=
+{ dom_of_dom := λ a, by simp [with_time],
+  some_of_some := λ ⟨t₁, a⟩ ⟨t₂, b⟩ h, 
+begin
+  apply reaches₁_single,
+  simp [with_time] at h,
+  rcases h with ⟨b', h, rfl, _⟩,
+  exact h,
+end,
+  none_of_none := λ ⟨t, a⟩, by simp [with_time] }
+
+theorem with_time_frespects_self {σ} (f : σ →. option σ) (n : ℕ) :
+  frespects (with_time f) (with_time f) (prod.map (+n) id) :=
+{ dom_of_dom := λ a, by simp [with_time],
+  some_of_some := λ ⟨t₁, a⟩ ⟨t₂, b⟩ h, 
+begin
+  apply reaches₁_single,
+  simp [with_time] at ⊢ h,
+  rcases h with ⟨b', h, rfl, ht⟩,
+  refine ⟨_, h, rfl, _⟩,
+  rw ← ht, ac_refl, 
+end,
+  none_of_none := λ ⟨t, a⟩, by simp [with_time] }
+
+end part_eval
